\documentclass{article}
\usepackage{amsmath,amssymb,amsthm}
\allowdisplaybreaks

\title{$\aleph_{0}$ Weekly Problem}
\author{Conrad Warren \and Ravi Dayabhai}
\date{2024-08-27}

\begin{document}

\maketitle

\section*{Problem}

Show that each number in the sequence $49, 4489, 444889, \ldots$ is a perfect square.

\section*{Solution}

\begin{proof}

The $n$th number in the sequence is given by $\left(\sum_{i=1}^{2n}4 \cdot 10^{i-1}\right) + \left(\sum_{i = 1}^{n} 4\cdot 10^{i-1}\right) + 1$. We will show that for any $n \in \lbrace 1, 2, \ldots \rbrace$, the $n$th term in the sequence equals a perfect square, namely, $(\left(\sum_{i = 1}^{n} 6 \cdot 10^{i-1} \right) + 1)^2$.
    
    \begin{align*}
    \left(\left(\sum_{i = 1}^{n} 6 \cdot 10^{i-1}\right) + 1\right)^2 &= \left(\sum_{i=1}^{2n}4 \cdot 10^{i-1}\right) + \left(\sum_{i = 1}^{n} 4\cdot 10^{i-1}\right) + 1\\
    \left(\sum_{i = 1}^{n} 6 \cdot 10^{i-1}\right)^2 + 2\cdot\left(\sum_{i = 1}^{n} 6 \cdot 10^{i-1}\right) + 1 &= \sum_{i=1}^{2n}4 \cdot 10^{i-1} + \sum_{i = 1}^{n} 4\cdot 10^{i-1} + 1\\
    \left(\sum_{i = 1}^{n} 6 \cdot 10^{i-1}\right)^2 + \sum_{i = 1}^{n} 8 \cdot 10^{i-1} &= \sum_{i=1}^{2n}4 \cdot 10^{i-1}\\
    36\left(\sum_{i = 1}^{n}10^{i-1}\right)^2 + 8\sum_{i = 1}^{n}10^{i-1} &= 4\sum_{i=1}^{2n}10^{i-1}\\
    9\left(\sum_{i = 1}^{n}10^{i-1}\right)^2 + 2\sum_{i = 1}^{n}10^{i-1} &= \sum_{i=1}^{2n}10^{i-1}\\
    \displaybreak\\
    9\left(\sum_{i = 1}^{n}10^{i-1}\right)^2 + 2\sum_{i = 1}^{n}10^{i-1} &= 10^n\sum_{i=1}^{n}10^{i-1} + \sum_{i=1}^{n}10^{i-1}\\
    9\left(\sum_{i = 1}^{n}10^{i-1}\right)^2 + \sum_{i = 1}^{n}10^{i-1} &= 10^n\sum_{i=1}^{n}10^{i-1}\\
    9\left(\sum_{i = 1}^{n}10^{i-1}\right) + 1 &= 10^n\\
    9\left(\sum_{i = 1}^{n}10^{i-1}\right) &= 10^n - 1 = 9\left(\sum_{i = 1}^{n}10^{i-1}\right)
    \end{align*}

By establishing the above equality, we have shown, for any index $n \in \lbrace 1, 2, \ldots \rbrace$, that the $n$th number in the given sequence is a perfect square of the form $(\left(\sum_{i = 1}^{n} 6 \cdot 10^{i-1} \right) + 1)^2$.

\end{proof}
\end{document}
